Test/civl/regression-tests/linear/allocator.bpl
@@ -1,15 +1,10 @@
 // RUN: %parallel-boogie "%s" > "%t"
 // RUN: %diff "%s.expect" "%t"
 
-
-
-
-type {:linear "tid"} X = int;
-
-procedure A({:linear_in "tid"} i': int) returns ({:linear "tid"} i: int);
+procedure A({:linear_in} i': int) returns ({:linear} i: int);
   ensures i == i';
 
-procedure B({:linear_in "tid"} i': int) returns ({:linear "tid"} i: int)
+procedure B({:linear_in} i': int) returns ({:linear} i: int)
 {
   i := i';
   call i := A(i);
