Test/civl/regression-tests/linear/bug.bpl
@@ -1,9 +1,7 @@
 // RUN: %parallel-boogie "%s" > "%t"
 // RUN: %diff "%s.expect" "%t"
 
-type {:linear ""} X = int;
-
-var {:linear ""} g:int;
+var {:linear} g:int;
 
 procedure A()
 {
