Test/civl/regression-tests/linear/f2.bpl
@@ -1,23 +1,16 @@
-// RUN: %parallel-boogie "%s" > "%t"
+// RUN: %parallel-boogie -lib:base "%s" > "%t"
 // RUN: %diff "%s.expect" "%t"
 
-
-
-
-
-
-type {:linear "1"} X = int;
-
-procedure Split({:linear_in "1"} xls: [int]bool) returns ({:linear "1"} xls1: [int]bool, {:linear "1"} xls2: [int]bool);
+procedure Split({:linear_in} xls: [int]bool) returns ({:linear} xls1: [int]bool, {:linear} xls2: [int]bool);
 ensures xls == MapOr(xls1, xls2) && xls1 != MapConst(false) && xls2 != MapConst(false);
 
-procedure Allocate() returns ({:linear "1"} x: [int]bool);
+procedure Allocate() returns ({:linear} x: [int]bool);
 
 procedure main()
 {
-   var {:linear "1"} x: [int] bool;
-   var {:linear "1"} x1: [int] bool;
-   var {:linear "1"} x2: [int] bool;
+   var {:linear} x: [int] bool;
+   var {:linear} x1: [int] bool;
+   var {:linear} x2: [int] bool;
 
    call x := Allocate();
    assume x == MapConst(true);
