Test/civl/regression-tests/yield-pre-post-mover.bpl
@@ -1,0 +1,26 @@
+// RUN: %parallel-boogie "%s" > "%t"
+// RUN: %diff "%s.expect" "%t"
+
+var {:layer 0,2} g: int;
+
+yield invariant {:layer 1} YieldInv#1();
+
+yield invariant {:layer 2} YieldInv#2();
+
+yield left procedure {:layer 2} A()
+requires {:layer 1} g > 0;
+preserves {:layer 1} g > 0;
+ensures {:layer 1} g > 0;
+requires {:layer 1,2} g > 0;
+preserves {:layer 1,2} g > 0;
+ensures {:layer 1,2} g > 0;
+requires {:layer 2} g > 0;
+preserves {:layer 2} g > 0;
+ensures {:layer 2} g > 0;
+requires call YieldInv#1();
+ensures call YieldInv#1();
+preserves call YieldInv#1();
+requires call YieldInv#2();
+ensures call YieldInv#2();
+preserves call YieldInv#2();
+{}
