Test/civl/regression-tests/yield-requires-ensures-errors-4.bpl
@@ -1,15 +1,15 @@
 // RUN: %parallel-boogie "%s" > "%t"
 // RUN: %diff "%s.expect" "%t"
 
-type {:linear "lin"} X = int;
+type {:linear} X = int;
 
 var {:layer 0,1} x:int;
 
-yield invariant {:layer 1} linear_yield_x({:linear "lin"} n: int);
+yield invariant {:layer 1} linear_yield_x({:linear} n: int);
 preserves x >= n;
 
 yield procedure {:layer 1}
-p3({:linear "lin"} a: int, {:linear_in "lin"} b: int, {:linear_out "lin"} c: int);
+p3({:linear} a: int, {:linear_in "lin"} b: int, {:linear_out "lin"} c: int);
 requires call linear_yield_x(a);
 ensures call linear_yield_x(a);
 requires call linear_yield_x(c);
