Test/civl/regression-tests/yield-requires-ensures-errors-5.bpl
@@ -1,15 +1,14 @@
 // RUN: %parallel-boogie "%s" > "%t"
 // RUN: %diff "%s.expect" "%t"
 
-type {:linear} X = int;
-
 var {:layer 0,1} x:int;
 
 yield invariant {:layer 1} yield_x(n: int);
 preserves x >= n;
 
-yield procedure {:layer 1} p2({:layer 0,0} a: int) returns (c: int)
+yield atomic procedure {:layer 1} p2(a: int) returns (c: int)
 requires call yield_x(a);
+preserves call yield_x(a);
 ensures call yield_x(a + c);
 {
 }
